---
title: Equation Index
description: ''
date: '2021-04-20T22:06:12.601Z'
venue: Equation Index
---

```{math}
:label: f4385f45

s=\frac{1}{v}
```

```{math}
:label: 0e35ead3

\rho = 1/\sigma
```

```{math}
:label: 3f2ba4e6

\mu = \mu_0 (1 + \kappa)
```

```{math}
:label: 77e80a1d

\mathcal{F}[m] = d
```

```{math}
:label: 3ffde9a8

d_j=\mathcal{F}_j[m]
```

```{math}
:label: ec8a3fad

\mathcal{F}[\alpha f+\beta g]=\alpha\mathcal{F}[f]+\beta\mathcal{F}[g]
```

```{math}
:label: f40ae85f

d_j=\int^b_ag_j(x)m(x)dx
```

```{math}
:label: c61a0203

y = m \otimes w
```

```{math}
:label: a7524253

y(t_j)=\int^{\infty}_{-\infty}m(\tau)w(t_j-\tau)d\tau
```

```{math}
:label: 32fe3486

\vec{B}(\vec{r}_j)=\frac{\mu_0}{4\pi}\int\frac{\vec{J}(\vec{r}\prime)\times\hat{r}}{\left|\vec{r}_j-\vec{r}\prime\right|^2}
```

```{math}
:label: 9e1acfa8

d_j^{(1)}=\int^b_a g_j(x)m_1(x)dx
```

```{math}
:label: 89373b07

d_j^{(2)}=\int^b_a g_j(x)m_2(x)dx
```

```{math}
:label: fc8ce57f

\begin{aligned}d_j=\int^b_a g_j(x)[\alpha & m_1(x) +\beta m_2(x)]\\ d_j=\alpha &d_j^{(1)}+\beta d_j^{(2)}\end{aligned}
```

```{math}
:label: 7f61dce7

d_j=\int^b_ag_j(x)m^2(x)dx
```

```{math}
:label: 0c8e0714

\nabla\cdot\sigma\nabla V=-I\delta(\vec{r}-\vec{r}\prime)
```

```{math}
:label: a19b615c

V^2_{rms}(t_j)=\frac{1}{t_j}\int^{t_{max}}_0 v^2_{int}(u)H(t_j-u)du
```

```{math}
:label: cc63b0e8

V^2_{rms}(t)=\frac{1}{t}\int^{t_{max}}_0 v_{int}^2(u)H(t-u)du
```

```{math}
:label: 815dcec5

v_{int}=V_{rms}(t)\left(1+\frac{2tV'_{rms}(t)}{V_{rms}(t)}\right)^{\frac{1}{2}}
```

```{math}
:label: c2de4591

V_{rms}(t)=v_0+a\sin(2\pi ft)
```

```{math}
:label: 2f6367b7

V'_{rms}(t)=2\pi af\cos(2\pi ft)
```

```{math}
:label: 1bc2c17d

d^{obs}=d^{true}+\delta d
```

```{math}
:label: d73ceb50

\mathcal{F}^{-1}[d^{true}]=m_c
```

```{math}
:label: 5c78d503

\mathcal{F}^{-1}[d^{obs}]=\mathcal{F}^{-1}[d^{true}+\delta d]=m_c+\delta m
```

```{math}
:label: ec61be48

\delta v_{int}\propto \sqrt{\frac{fta}{v_0}}
```

```{math}
:label: d44e43b7

P(m|d^{obs})\propto P(d^{obs}|m)P(m)
```

```{math}
:label: 7633cf80

\begin{aligned}&\text{Minimize}~~\phi=\phi_d+\beta\phi_m\\ &\text{subject to}~~m_l<m<m_u,\end{aligned}
```

```{math}
:label: 4f6a44b9

g_j(x)= e^{p_jx}\cos(2\pi q_jx)
```

```{math}
:label: be6adec9

\begin{aligned} d_j&=\int_0^{x_1}g_j(x)m_1dx +\int_{x_1}^{x_2}g_j(x)m_2dx+\dots \\ &=\sum^M_{i=1}\left(\int_{x_{k-1}}^{x_k}g_j\left(x\right)dx\right)m_i\\ &\\ d_j &= \mathbf g_j \mathbf m\end{aligned}
```

```{math}
:label: d031bcf8

\begin{aligned} \mathbf{d} = \mathbf{G}\mathbf{m} = \begin{bmatrix} d_1\\ \vdots\\ d_{N} \end{bmatrix}\end{aligned}
```

```{math}
:label: 2664f2ef

G_{jk} = \int_{x_{k-1}}^{x_k} g_j(x) dx
```

```{math}
:label: adc69a91

\mathbf{d}^{obs}=\mathbf{d}+\mathbf{n}
```

```{math}
:label: 9e813186

\epsilon_j = \%|d_j| + \nu_j
```

```{math}
:label: 9424a329

\phi_d=\sum^N_{j=1}\left(\frac{d_j-d_j^{obs}}{\epsilon_j}\right)^2
```

```{math}
:label: c93bd419

\eta_j = \frac {d_j - d_j^{obs}} {\epsilon_j}
```

```{math}
:label: 198b31c2

E[\chi^2] = N
```

```{math}
:label: 000e5f6c

Var[\chi^2] = 2N
```

```{math}
:label: 8e0a1ed0

\phi_d^*=N
```

```{math}
:label: 5bb81c63

\phi_m=\int (m-m^{ref})^2 dx
```

```{math}
:label: dd987b9d

\phi_m=\int \left(\frac{d(m-m^{ref})}{dx}\right)^2 dx
```

```{math}
:label: 05257042

\phi_m=\alpha_s\int (m-m^{ref})^2 dx+\alpha_x\int (\frac{d(m-m^{ref})}{dx})^2 dx
```

```{math}
:label: 64af53ab

\phi_m=\|\mathbf{m - m^{ref}}\|^2=\sum_{i=1}^M(m_i-m^{ref}_i)^2
```

```{math}
:label: 8242954b

\phi_m=\|\frac{d\mathbf{m}}{dx}\|^2=\sum_{i=1}^{M-1}(m_{i+1}-m_i)^2
```

```{math}
:label: fd471526

\phi(m) = \phi_d(m)+\beta\phi_m(m)
```

```{math}
:label: 7c304ef3

\phi=T+\beta F
```

$$\mathbf{g}_j(\mathbf{x}) = e^{p_j\mathbf{x}} cos (2 \pi q_j \mathbf{x}) \Delta x$$

```{math}
:label: 8839db7e

\begin{aligned} \mathbf{G} = \begin{bmatrix} \mathbf{g}_1\\ \vdots\\ \mathbf{g}_{N} \end{bmatrix} \end{aligned}
```
